WIP -- let's use id instead of fptr
Rationale: one can always translate fptr into id using skenv_link

theories/ModSem.v
@@ -1,34 +1,76 @@
-From Paco Require Import paco.
-Require Import Program.
-Require Import sflib.
+Require Import Coqlib.
+Require Import ITreelib.
 Require Import Universe.
-Require Import STS.
-Require Import Behavior.
 Require Import Skeleton.
+Require Import PCM.
 
 Set Implicit Arguments.
 
 
 
-(* Module ModSem. *)
+Module ModSem.
+Section MODSEM.
 
-(*   Inductive sort: Type := *)
-(*   | angelic *)
-(*   | demonic *)
-(*   | final (retv: val) *)
-(*   | vis *)
-(*   | at_external (args: list val) *)
-(*   . *)
+  (* Record t: Type := mk { *)
+  (*   state: Type; *)
+  (*   local_data: Type; *)
+  (*   step (skenv: SkEnv.t) (st0: state) (ev: option event) (st1: state): Prop; *)
+  (*   state_sort: state -> sort; *)
+  (*   initial_local_data: local_data; *)
+  (*   sk: Sk.t; *)
+  (*   name: string; *)
+  (* } *)
+  (* . *)
 
-(*   Record t: Type := mk { *)
-(*     state: Type; *)
-(*     local_data: Type; *)
-(*     step (skenv: SkEnv.t) (st0: state) (ev: option event) (st1: state): Prop; *)
-(*     state_sort: state -> sort; *)
-(*     initial_local_data: local_data; *)
-(*     sk: Sk.t; *)
-(*     name: string; *)
-(*   } *)
-(*   . *)
+  Inductive eventE: Type -> Type :=
+  | Choose X: eventE X
+  | Take X: eventE X
+  .
 
-(* End ModSem. *)
+  Context `{GRA: GRA.t}.
+
+  Inductive callE: Type -> Type :=
+  | Call (fptr: val) (args: list val): callE val
+  .
+
+  Inductive ldE: Type -> Type :=
+  | LPut (r: (GRA.construction GRA)): ldE unit
+  | LGet: ldE (GRA.construction GRA)
+  .
+
+  Record t: Type := mk {
+    sk: Sk.t;
+    initial_ld: GRA.construction GRA;
+    sem: callE ~> itree (callE +' ldE);
+  }
+  .
+
+  Definition wf (md: t): Prop := Sk.wf md.(sk).
+
+  (*** using "Program Definition" makes the definition uncompilable; why?? ***)
+  Definition merge (md0 md1: t): t := {|
+    sk := Sk.add md0.(sk) md1.(sk);
+    initial_ld := URA.add md0.(initial_ld) md1.(initial_ld);
+    (* sem := fun _ c => match c with *)
+    (*                   | call fptr args => md0.(sem) (call fptr args) *)
+    (*                   end *)
+    sem := fun _ '(Call fptr args) =>
+             if md0.(sk) md0.(sem) (Call fptr args);
+  |}
+  .
+
+End MODSEM.
+End ModSem.
+
+Inductive ModSem: Type :=
+  mk_ModSem { fnames: string -> bool ;
+              owned_heap: Type;
+              initial_owned_heap: owned_heap;
+              customE: Type -> Type ;
+              handler: customE ~> stateT owned_heap (itree (GlobalE +' Event));
+
+              (* handler: forall E, AnyState ~> stateT Any (itree E); *)
+              (* sem: CallExternalE ~> itree (CallExternalE +' Event); *)
+
+              sem: CallExternalE ~> itree (CallExternalE +' customE +' GlobalE +' Event);
+            }.
