theories/Universe.v
@@ -1,17 +1,18 @@
 Require Export ZArith.
 Require Export String.
 
-Notation block := positive (only parsing).
+Notation block := nat (only parsing).
 
 Inductive val: Type :=
 | Vint (n: Z): val
-| Vptr (blk: block) (ofs: Z): val 
+| Vptr (blk: block) (ofs: Z): val
+| Vundef
 .
 
-Notation ident := positive (only parsing).
+Notation ident := string (only parsing).
 
 Inductive event: Type :=
 | event_sys
-    (name: string)
+    (name: ident)
     (args: list val)
 .
